examples/layeredeffects/ID5.fst
@@ -46,7 +46,7 @@ irreducible let refine : unit = ()
 let subcomp (a:Type u#uu) (w1 w2:wp a)
     (f : repr a w1)
 : Pure (repr a w2)
-       (requires forall p. w2 p ==> w1 p)
+       (requires forall p. {:nopattern} w2 p ==> w1 p)
        (ensures fun _ -> True)
 = f
 
@@ -111,7 +111,7 @@ effect {
 }
 
 effect Id (a:Type) (pre:Type0) (post:a->Type0) =
-        ID a (as_pure_wp (fun p -> pre /\ (forall x. post x ==> p x)))
+        ID a (as_pure_wp (fun p -> pre /\ (forall x. {:nopattern} post x ==> p x)))
 
 effect I (a:Type) = Id a True (fun _ -> True)
 
@@ -151,7 +151,7 @@ let rec map #a #b #pre
   (f : (x:a -> Id b (requires (pre x)) (ensures (fun _ -> True))))
   (l : list a)
   : Id (list b)
-       (requires (forall x. memP x l ==> pre x))
+       (requires (forall x. {:nopattern} memP x l ==> pre x))
        (ensures (fun _ -> True))
   = match l with
     | [] -> []
