src/parser/FStarC.Parser.Dep.fst
@@ -951,9 +951,9 @@ let collect_module_or_decls (filename:string) (m:either modul (list decl)) : ML 
           | Inr t -> collect_term t)
           binders;
         collect_term t
-    | QForall (binders, (_, ts), t)
-    | QExists (binders, (_, ts), t)
-    | QuantOp (_, binders, (_, ts), t) ->
+    | QForall (binders, (_, ts, _), t)
+    | QExists (binders, (_, ts, _), t)
+    | QuantOp (_, binders, (_, ts, _), t) ->
         collect_binders binders;
         List.iter (List.iter collect_term) ts;
         collect_term t
